Basic Termination Result for Trees

ProofLibrary/PossiblyInfiniteTree.lean
@@ -8,13 +8,43 @@ import ProofLibrary.PossiblyInfiniteList
 def InfiniteTreeSkeleton (α : Type u) := (List Nat) -> α
 
 namespace InfiniteTreeSkeleton
+
   def children (tree : InfiniteTreeSkeleton α) (node : List Nat) : InfiniteList α := fun n => tree (n :: node)
 
-  def branches (tree : InfiniteTreeSkeleton α) : Set (InfiniteList α) := fun branch =>
-    ∃ nodes : InfiniteList Nat, ∀ n : Nat, branch n = tree (nodes.take n).reverse
-
   def branches_through (tree : InfiniteTreeSkeleton α) (node : List Nat) : Set (InfiniteList α) := fun branch =>
-    branch ∈ tree.branches ∧ ∀ (i : Fin (node.length + 1)), branch i = tree (node.drop (node.length-i))
+    ∃ nodes : InfiniteList Nat, (∀ n : Nat, branch n = tree (nodes.take n).reverse) ∧ (nodes.take node.length).reverse = node
+
+  def branches (tree : InfiniteTreeSkeleton α) : Set (InfiniteList α) := tree.branches_through []
+
+  theorem branches_through_eq_union_children (tree : InfiniteTreeSkeleton α) (node : List Nat) : tree.branches_through node = fun b => ∃ (i : Nat), b ∈ tree.branches_through (i :: node) := by
+    unfold branches_through
+    apply funext
+    simp
+    intro b
+    constructor
+    . intro ⟨nodes, h⟩
+      exists nodes node.length
+      simp [Set.element]
+      exists nodes
+      constructor
+      . exact h.left
+      . unfold InfiniteList.take
+        simp
+        rw [← List.reverse_eq_iff]
+        exact h.right
+    . intro h
+      rcases h with ⟨i, nodes, h⟩
+      exists nodes
+      constructor
+      . exact h.left
+      . have hr := h.right
+        unfold InfiniteList.take at hr
+        rw [← List.reverse_inj] at hr
+        rw [List.reverse_append] at hr
+        rw [List.reverse_append] at hr
+        simp at hr
+        exact hr.right
+
 end InfiniteTreeSkeleton
 
 structure PossiblyInfiniteTree (α : Type u) where
@@ -82,11 +112,25 @@ namespace PossiblyInfiniteTree
     unfold InfiniteTreeSkeleton.children
     simp
 
+  def branches_through (tree : PossiblyInfiniteTree α) (node : List Nat) : Set (PossiblyInfiniteList α) := fun pil =>
+    pil.infinite_list ∈ tree.infinite_tree.branches_through node
+
   def branches (tree : PossiblyInfiniteTree α) : Set (PossiblyInfiniteList α) := fun pil =>
     pil.infinite_list ∈ tree.infinite_tree.branches
 
-  def branches_through (tree : PossiblyInfiniteTree α) (node : List Nat) : Set (PossiblyInfiniteList α) := fun pil =>
-    pil.infinite_list ∈ tree.infinite_tree.branches_through node
+  theorem branches_through_eq_union_children (tree : PossiblyInfiniteTree α) (node : List Nat) : tree.branches_through node = fun b => ∃ (i : Nat), b ∈ tree.branches_through (i :: node) := by
+    unfold branches_through
+    apply funext
+    simp
+    intro pil
+    rw [tree.infinite_tree.branches_through_eq_union_children]
+    constructor
+    . intro h
+      rcases h with ⟨i, h⟩
+      exists i
+    . intro h
+      rcases h with ⟨i, h⟩
+      exists i
 
   def leaves (tree : PossiblyInfiniteTree α) : Set α := fun a => ∃ node : List Nat, tree.get node = some a ∧ tree.children node = PossiblyInfiniteList.empty
 end PossiblyInfiniteTree
@@ -389,10 +433,377 @@ namespace FiniteDegreeTree
     rw [PossiblyInfiniteList.get_fromList_eq_list_getElem]
     apply getElem_children_eq_getElem_tree_children
 
-  def branches (tree : FiniteDegreeTree α) : Set (PossiblyInfiniteList α) := tree.tree.branches
-
   def branches_through (tree : FiniteDegreeTree α) (node : List Nat) : Set (PossiblyInfiniteList α) := tree.tree.branches_through node
 
+  def branches (tree : FiniteDegreeTree α) : Set (PossiblyInfiniteList α) := tree.tree.branches
+
+  theorem branches_through_eq_union_children (tree : FiniteDegreeTree α) (node : List Nat) : tree.branches_through node = fun b => ∃ (i : Nat), b ∈ tree.branches_through (i :: node) := by
+    unfold branches_through
+    rw [tree.tree.branches_through_eq_union_children]
+
   def leaves (tree : FiniteDegreeTree α) : Set α := tree.tree.leaves
+
+  theorem branches_through_finite_of_none (tree : FiniteDegreeTree α) (node : List Nat) : tree.get node = none -> (tree.branches_through node).finite := by
+    intro is_none
+    let branch_for_node : PossiblyInfiniteList α := ⟨fun n => if n ≤ node.length then tree.get (node.drop (node.length - n)) else none, by
+      intro n not_none
+      cases Decidable.em (n ≤ node.length) with
+      | inr lt => simp [lt] at not_none
+      | inl le =>
+        simp [le] at not_none
+        intro m
+        have m_le : m ≤ node.length := by apply Nat.le_trans; apply Nat.le_of_lt m.isLt; exact le
+        simp [m_le]
+        have no_orphans := tree.tree.no_orphans (node.drop (node.length - n)) not_none ⟨(node.drop (node.length - m)), by
+          exists (node.drop (node.length - n)).take (n - m)
+          rw [List.take_drop]
+          have : node.length - n + (n - m.val) = node.length - m.val := by
+            rw [← Nat.add_sub_assoc (by apply Nat.le_of_lt; exact m.isLt)]
+            rw [← Nat.sub_add_comm le]
+            simp
+          rw [this]
+          rw [← List.drop_append_of_le_length (by rw [List.length_take_of_le (by simp), Nat.sub_le_sub_iff_left m_le]; apply Nat.le_of_lt; exact m.isLt)]
+          simp
+        ⟩
+        exact no_orphans
+    ⟩
+    exists [branch_for_node]
+    constructor
+    . simp
+    . intro e
+      constructor
+      . intro h
+        simp at h
+        rw [h]
+        let nodes : InfiniteList Nat := fun n => if lt : n < node.length then node[node.length - (n+1)] else (tree.children node).length
+        have : ∀ n, n ≤ node.length -> (nodes.take n).reverse = node.drop (node.length - n) := by
+          intro n
+          induction n with
+          | zero => simp [InfiniteList.take]
+          | succ n ih =>
+            intro le
+            unfold InfiniteList.take
+            simp
+            rw [ih (by apply Nat.le_of_succ_le le)]
+            unfold nodes
+            have lt : n < node.length := by apply Nat.lt_of_succ_le le
+            simp [lt]
+            conv => right; rw [List.drop_eq_getElem_cons (by apply Nat.sub_lt_self; simp; exact le)]
+            have : node.length - (n + 1) + 1 = node.length - n := by omega
+            rw [this]
+        exists nodes
+        constructor
+        . intro n
+          cases Decidable.em (n ≤ node.length) with
+          | inl le =>
+            rw [this n le]
+            simp [le]
+            rfl
+          | inr lt =>
+            simp [lt]
+            have no_orphans := tree.tree.no_orphans (nodes.take n).reverse
+            apply Eq.symm
+            apply Option.decidable_eq_none.byContradiction
+            intro contra
+            specialize no_orphans contra ⟨node, by
+              exists ((nodes.skip (node.length)).take (n - node.length)).reverse
+              have : node = (nodes.take (node.length)).reverse := by
+                rw [this node.length]
+                . simp
+                . simp
+              conv => left; right; rw [this]
+              rw [← List.reverse_append]
+              rw [InfiniteList.combine_skip_take nodes n ⟨node.length, by apply Nat.lt_of_not_le; exact lt⟩]
+            ⟩
+            apply no_orphans
+            exact is_none
+        . rw [this]
+          . simp
+          . simp
+      . intro h
+        rcases h with ⟨nodes, h⟩
+        simp
+        rw [PossiblyInfiniteList.eq_iff_same_on_all_indices]
+        intro n
+        rw [h.left]
+        unfold branch_for_node
+        simp
+        cases Decidable.em (n ≤ node.length) with
+        | inl le =>
+          simp [le]
+          have : (nodes.take n).reverse = node.drop (node.length - n) := by
+            conv => right; right; rw [← h.right]
+            rw [List.drop_reverse]
+            rw [InfiniteList.length_take]
+            rw [InfiniteList.take_after_take]
+            rw [Nat.sub_sub_self le]
+            simp [Nat.min_eq_right le]
+          rw [this]
+          rfl
+        | inr lt =>
+          simp [lt]
+
+          have no_orphans := tree.tree.no_orphans (nodes.take n).reverse
+          apply Option.decidable_eq_none.byContradiction
+          intro contra
+          specialize no_orphans contra ⟨node, by
+            exists ((nodes.skip (node.length)).take (n - node.length)).reverse
+            conv => left; right; rw [← h.right]
+            rw [← List.reverse_append]
+            rw [InfiniteList.combine_skip_take nodes n ⟨node.length, by apply Nat.lt_of_not_le; exact lt⟩]
+          ⟩
+          apply no_orphans
+          exact is_none
+
+  theorem branches_through_finite_of_branches_through_children_finite (tree : FiniteDegreeTree α) (node : List Nat) : (∀ i, (tree.branches_through (i :: node)).finite) -> (tree.branches_through node).finite := by
+    intro h
+    have dec := Classical.typeDecidableEq (PossiblyInfiniteList α)
+    let branch_for_node : PossiblyInfiniteList α := ⟨fun n => if n ≤ node.length then tree.get (node.drop (node.length - n)) else none, by
+      intro n not_none
+      cases Decidable.em (n ≤ node.length) with
+      | inr lt => simp [lt] at not_none
+      | inl le =>
+        simp [le] at not_none
+        intro m
+        have m_le : m ≤ node.length := by apply Nat.le_trans; apply Nat.le_of_lt m.isLt; exact le
+        simp [m_le]
+        have no_orphans := tree.tree.no_orphans (node.drop (node.length - n)) not_none ⟨(node.drop (node.length - m)), by
+          exists (node.drop (node.length - n)).take (n - m)
+          rw [List.take_drop]
+          have : node.length - n + (n - m.val) = node.length - m.val := by
+            rw [← Nat.add_sub_assoc (by apply Nat.le_of_lt; exact m.isLt)]
+            rw [← Nat.sub_add_comm le]
+            simp
+          rw [this]
+          rw [← List.drop_append_of_le_length (by rw [List.length_take_of_le (by simp), Nat.sub_le_sub_iff_left m_le]; apply Nat.le_of_lt; exact m.isLt)]
+          simp
+        ⟩
+        exact no_orphans
+    ⟩
+    let branches_for_i (i : Nat) := Classical.choose (h i)
+    let target_list : List (PossiblyInfiniteList α) := (branch_for_node :: ((tree.children node).enum_with_lt.map (fun (i, _) => branches_for_i i.val)).flatten).eraseDupsKeepRight
+    exists target_list
+    constructor
+    . apply List.nodup_eraseDupsKeepRight
+    . intro branch
+      unfold target_list
+      rw [List.mem_eraseDupsKeepRight_iff]
+      simp
+      constructor
+      . intro pre
+        cases pre with
+        | inl eq =>
+          let nodes : InfiniteList Nat := fun n => if lt : n < node.length then node[node.length - (n+1)] else (tree.children node).length
+          have : ∀ n, n ≤ node.length -> (nodes.take n).reverse = node.drop (node.length - n) := by
+            intro n
+            induction n with
+            | zero => simp [InfiniteList.take]
+            | succ n ih =>
+              intro le
+              unfold InfiniteList.take
+              simp
+              rw [ih (by apply Nat.le_of_succ_le le)]
+              unfold nodes
+              have lt : n < node.length := by apply Nat.lt_of_succ_le le
+              simp [lt]
+              conv => right; rw [List.drop_eq_getElem_cons (by apply Nat.sub_lt_self; simp; exact le)]
+              have : node.length - (n + 1) + 1 = node.length - n := by omega
+              rw [this]
+          exists nodes
+          constructor
+          . rw [eq]
+            intro n
+            cases Decidable.em (n ≤ node.length) with
+            | inl le =>
+              rw [this n le]
+              simp [le]
+              rfl
+            | inr lt =>
+              simp [lt]
+              have : tree.tree.infinite_tree (nodes.take (node.length + 1)).reverse = none := by
+                have child_none : (tree.children node)[nodes node.length]? = none := by
+                  apply List.getElem?_eq_none
+                  unfold nodes
+                  simp
+                rw [getElem_children_eq_getElem_tree_children, PossiblyInfiniteTree.getElem_children_eq_get_tree] at child_none
+                unfold PossiblyInfiniteTree.get at child_none
+                unfold InfiniteList.take
+                simp
+                rw [this]
+                . simp
+                  exact child_none
+                . simp
+              have le : node.length + 1 ≤ n := by apply Nat.succ_le_of_lt; apply Nat.lt_of_not_ge; exact lt
+              cases Nat.eq_or_lt_of_le le with
+              | inl eq => rw [← eq, this]
+              | inr lt =>
+                have no_orphans := tree.tree.no_orphans (nodes.take n).reverse
+                apply Eq.symm
+                apply Option.decidable_eq_none.byContradiction
+                intro contra
+                specialize no_orphans contra ⟨(nodes.take (node.length + 1)).reverse, by
+                  exists ((nodes.skip (node.length + 1)).take (n - (node.length + 1))).reverse
+                  rw [← List.reverse_append]
+                  rw [InfiniteList.combine_skip_take nodes n ⟨node.length + 1, lt⟩]
+                ⟩
+                apply no_orphans
+                exact this
+          . rw [this]
+            . simp
+            . simp
+        | inr pre =>
+          rcases pre with ⟨branches, ex_i, branch_mem⟩
+          rcases ex_i with ⟨i, _, eq⟩
+          rw [branches_through_eq_union_children]
+          exists i.val
+          have spec := Classical.choose_spec (h i.val)
+          rw [← spec.right]
+          unfold branches_for_i at eq
+          rw [eq]
+          exact branch_mem
+      . intro pre
+        rw [branches_through_eq_union_children] at pre
+        rcases pre with ⟨i, pre⟩
+        cases Decidable.em (i < (tree.children node).length) with
+        | inl lt =>
+          apply Or.inr
+          exists branches_for_i i
+          constructor
+          . let i_fin : Fin (tree.children node).length := ⟨i, lt⟩
+            exists i_fin
+            constructor
+            . exists (tree.children node)[i_fin]
+              rw [List.mem_enum_with_lt_iff_mem_enum]
+              rw [List.mem_enum_iff_getElem?]
+              simp
+            . rfl
+          . have spec := Classical.choose_spec (h i)
+            unfold branches_for_i
+            rw [spec.right]
+            exact pre
+        | inr not_lt =>
+          apply Or.inl
+          rcases pre with ⟨nodes, pre⟩
+          unfold branch_for_node
+          rw [PossiblyInfiniteList.eq_iff_same_on_all_indices]
+          intro n
+          rw [pre.left n]
+          have pre_r := pre.right
+          simp [InfiniteList.take] at pre_r
+          simp
+          cases Decidable.em (n ≤ node.length) with
+          | inl le =>
+            simp [le]
+            have : (nodes.take n).reverse = node.drop (node.length - n) := by
+              conv => right; right; rw [← pre_r.right]
+              rw [List.drop_reverse]
+              rw [InfiniteList.length_take]
+              rw [InfiniteList.take_after_take]
+              rw [Nat.sub_sub_self le]
+              simp [Nat.min_eq_right le]
+            rw [this]
+            rfl
+          | inr lt =>
+            simp [lt]
+            have : tree.tree.infinite_tree (nodes.take (node.length + 1)).reverse = none := by
+              have : (tree.children node)[nodes node.length]? = none := by
+                apply List.getElem?_eq_none
+                rw [pre_r.left]
+                apply Nat.le_of_not_gt
+                exact not_lt
+              rw [getElem_children_eq_getElem_tree_children, PossiblyInfiniteTree.getElem_children_eq_get_tree] at this
+              unfold PossiblyInfiniteTree.get at this
+              unfold InfiniteList.take
+              simp
+              rw [pre_r.right]
+              exact this
+            have le : node.length + 1 ≤ n := by apply Nat.succ_le_of_lt; apply Nat.lt_of_not_ge; exact lt
+            cases Nat.eq_or_lt_of_le le with
+            | inl eq => rw [← eq]; exact this
+            | inr lt =>
+              have no_orphans := tree.tree.no_orphans (nodes.take n).reverse
+              apply Option.decidable_eq_none.byContradiction
+              intro contra
+              specialize no_orphans contra ⟨(nodes.take (node.length + 1)).reverse, by
+                exists ((nodes.skip (node.length + 1)).take (n - (node.length + 1))).reverse
+                rw [← List.reverse_append]
+                rw [InfiniteList.combine_skip_take nodes n ⟨node.length + 1, lt⟩]
+              ⟩
+              apply no_orphans
+              exact this
+
+  noncomputable def infinite_branching_node_for_depth_of_branches_infinite (tree : FiniteDegreeTree α) (not_finite : ¬ tree.branches.finite) : (depth : Nat) -> { node : List Nat // node.length = depth ∧ ¬ (tree.branches_through node).finite }
+  | .zero => ⟨[], by constructor; rfl; exact not_finite⟩
+  | .succ depth =>
+    let prev_res := infinite_branching_node_for_depth_of_branches_infinite tree not_finite depth
+    let prev_node := prev_res.val
+    let length_eq := prev_res.property.left
+    let not_finite := prev_res.property.right
+    have : ¬ ∀ i, (tree.branches_through (i :: prev_node)).finite := by
+      intro contra
+      apply not_finite
+      apply branches_through_finite_of_branches_through_children_finite
+      exact contra
+    have : ∃ i, ¬ (tree.branches_through (i :: prev_node)).finite := by simp at this; exact this
+    let i := Classical.choose this
+    let i_spec := Classical.choose_spec this
+
+    ⟨i :: prev_node, by
+      constructor
+      . simp; exact length_eq
+      . exact i_spec
+    ⟩
+
+  theorem infinite_branching_node_extends_previous (tree : FiniteDegreeTree α) (not_finite : ¬ tree.branches.finite) (depth : Nat) : (infinite_branching_node_for_depth_of_branches_infinite tree not_finite depth.succ).val = (infinite_branching_node_for_depth_of_branches_infinite tree not_finite depth.succ).val.head (by simp [infinite_branching_node_for_depth_of_branches_infinite]) :: (infinite_branching_node_for_depth_of_branches_infinite tree not_finite depth).val := by
+    simp [infinite_branching_node_for_depth_of_branches_infinite]
+
+  theorem branches_finite_of_each_finite (tree : FiniteDegreeTree α) : (∀ branch, branch ∈ tree.branches -> ∃ i, branch.infinite_list i = none) -> tree.branches.finite := by
+    intro h
+
+    apply Classical.byContradiction
+    intro contra
+    simp at contra
+
+    have : ∃ (nodes : InfiniteList Nat), ∀ (i : Nat), ¬ (tree.branches_through (nodes.take i).reverse).finite := by
+      let nodes : InfiniteList Nat := fun n => (infinite_branching_node_for_depth_of_branches_infinite tree contra n.succ).val.head (by
+        simp [infinite_branching_node_for_depth_of_branches_infinite]
+      )
+      have : ∀ i, (nodes.take i).reverse = (infinite_branching_node_for_depth_of_branches_infinite tree contra i).val := by
+        intro i
+        induction i with
+        | zero => simp [InfiniteList.take, infinite_branching_node_for_depth_of_branches_infinite]
+        | succ i ih =>
+          unfold InfiniteList.take
+          unfold nodes
+          simp
+          rw [ih]
+          conv => right; rw [infinite_branching_node_extends_previous]
+      exists nodes
+      intro i
+      rw [this]
+      have prop := (infinite_branching_node_for_depth_of_branches_infinite tree contra i).property
+      exact prop.right
+
+    rcases this with ⟨nodes, all_infinite⟩
+
+    let branch : PossiblyInfiniteList α := ⟨fun n => tree.get (nodes.take n).reverse, by
+      intro n not_none m contra
+      apply all_infinite m.val
+      apply branches_through_finite_of_none
+      exact contra
+    ⟩
+
+    specialize h branch (by
+      exists nodes
+      constructor
+      . intro n
+        rfl
+      . rfl
+    )
+
+    rcases h with ⟨i, hi⟩
+    apply all_infinite i
+    apply branches_through_finite_of_none
+    exact hi
 end FiniteDegreeTree
 
