ProofLibrary/PossiblyInfiniteList.lean
@@ -7,6 +7,9 @@ namespace InfiniteList
   | 0 => []
   | n+1 => (l.take n) ++ [l n]
 
+  theorem length_take (l : InfiniteList α) (n : Nat) : (l.take n).length = n := by
+    induction n ; simp [take] ; simpa [take]
+
   def skip (l : InfiniteList α) (m : Nat) : InfiniteList α := fun n => l (n + m)
 
   theorem skip_zero_eq (l : InfiniteList α) : l.skip 0 = l := by unfold skip; simp only [Nat.add_zero]
@@ -39,6 +42,30 @@ namespace InfiniteList
         have : m = k := by cases Nat.lt_or_eq_of_le (Nat.le_of_lt_succ m.isLt); contradiction; assumption
         rw [this]
         simp [take]
+
+  theorem take_after_take (l : InfiniteList α) (n m : Nat) : (l.take n).take m = l.take (n.min m) := by
+    induction n with
+    | zero => simp [take]
+    | succ n ih =>
+      simp [take]
+      rw [List.take_append_eq_append_take]
+      rw [ih]
+      rw [length_take]
+      cases Decidable.em (n ≤ m) with
+      | inl le =>
+        simp [Nat.min_eq_left le]
+        cases Nat.eq_or_lt_of_le le with
+        | inl eq =>
+          rw [eq]
+          simp
+        | inr lt =>
+          simp [Nat.min_eq_left (Nat.succ_le_of_lt lt)]
+          conv => right; unfold InfiniteList.take
+          rw [List.take_of_length_le (by apply Nat.le_sub_of_add_le; rw [Nat.add_comm, List.length_singleton]; apply Nat.succ_le_of_lt; exact lt)]
+      | inr lt =>
+        simp at lt
+        simp [Nat.min_eq_right (Nat.le_of_lt lt), Nat.min_eq_right (Nat.le_succ_of_le (Nat.le_of_lt lt))]
+        apply Nat.sub_eq_zero_of_le (Nat.le_of_lt lt)
 end InfiniteList
 
 @[ext]
